# 链式法则

对于复合函数$f(g(x))$，有$(f \circ g)^{\prime}(x)=f^{\prime}(g(x)) g^{\prime}(x)$。

## 证明

设$f$和$g$为函数，$x$为常数，使得$f$在$g(x)$可导，且$g$在$x$可导。根据可导的定义，

$\frac{g(x+\delta)-g(x)}{\delta} - g'(x) = \epsilon(\delta) \Rightarrow g(x+\delta)-g(x)= \delta g'(x) + \epsilon(\delta)\delta ,$，其中当$\delta\to 0$时，$ \epsilon(\delta) \to 0 \,$。

同理，

$ f(g(x)+\alpha) - f(g(x)) = \alpha f'(g(x)) + \eta(\alpha)\alpha \,$，其中当$\alpha\to 0$时，$\eta(\alpha) \to 0 \,$。

现在

$ f(g(x+\delta))-f(g(x)) = f(g(x) + \delta g'(x)+\epsilon(\delta)\delta) - f(g(x)) = \alpha_\delta f'(g(x)) + \eta(\alpha_\delta)\alpha_\delta \,$

其中$\alpha_\delta = \delta g'(x) + \epsilon(\delta)\delta \,$.

左右两式同除以$\delta$，有

$\frac{f(g(x + \delta)) - f(g(x))}{\delta} = \frac{\alpha_{\delta}}{\delta}f'(g(x)) + \frac{\eta(\alpha_{\delta})\alpha_{\delta}}{\delta}$

注意到当$\delta\to 0$时，$\frac{\alpha_\delta}{\delta}\to g'(x)$及$\alpha_\delta \to 0$，因此 $\eta(\alpha_\delta)\to 0$。故有

$ \frac{f(g(x+\delta))-f(g(x))}{\delta} \to g'(x)f'(g(x)).$